LeanSAT/Model/Map.lean
@@ -1,0 +1,122 @@
+/-
+Copyright (c) 2024 The LeanSAT Contributors.
+Released under the Apache License v2.0; see LICENSE for full text.
+
+Authors: James Gallicchio
+-/
+
+import LeanSAT.Model.PropFun
+import LeanSAT.Model.PropVars
+
+namespace LeanSAT.Model
+
+/-! ### `map` -/
+
+namespace PropForm
+
+@[simp]
+def map (f : ν₁ → ν₂) : PropForm ν₁ → PropForm ν₂
+| .var l => .var (f l)
+| .tr => .tr
+| .fls => .fls
+| .neg φ => .neg (map f φ)
+| .conj φ₁ φ₂ => .conj (map f φ₁) (map f φ₂)
+| .disj φ₁ φ₂ => .disj (map f φ₁) (map f φ₂)
+| .impl φ₁ φ₂ => .impl (map f φ₁) (map f φ₂)
+| .biImpl φ₁ φ₂ => .biImpl (map f φ₁) (map f φ₂)
+
+section map
+
+variable (f : ν₁ → ν₂) (φ φ₁ φ₂ : PropForm ν₁)
+
+@[simp]
+theorem vars_map [DecidableEq ν₁] [DecidableEq ν₂] : vars (φ.map f) = φ.vars.image f := by
+  induction φ <;> simp [*, Finset.image_union]
+
+theorem satisfies_map {φ : PropForm ν₁} {f} {τ : PropAssignment ν₂}
+    : τ ⊨ φ.map f ↔ (τ.map f) ⊨ φ := by
+  induction φ <;> (simp [map, PropAssignment.map] at *) <;> (simp [*])
+
+@[simp]
+theorem semVars_map [DecidableEq ν₁] [DecidableEq ν₂] [Fintype ν₁]
+      {f : ν₁ → ν₂} (hf : f.Injective) (φ : PropForm ν₁)
+    : PropFun.semVars ⟦φ.map f⟧ = (PropFun.semVars ⟦φ⟧).map ⟨f,hf⟩ := by
+  ext v2; simp
+  constructor
+  · intro h
+    have isVar : v2 ∈ vars (map f φ) := semVars_subset_vars _ h
+    simp at isVar
+    rcases isVar with ⟨v1, _, rfl⟩
+    simp [hf.eq_iff]
+    have := by rw [PropFun.mem_semVars] at h; exact h
+    rcases this with ⟨τ,hpos,hneg⟩
+    rw [PropFun.satisfies_mk] at hpos hneg
+    simp [satisfies_map] at hpos hneg
+    rw [PropAssignment.map_set (finj := hf)] at hneg
+    rw [PropFun.mem_semVars]
+    use PropAssignment.map f τ
+    simp
+    rw [PropFun.satisfies_mk, PropFun.satisfies_mk]; simp [*]
+  . rintro ⟨v1,hv1,rfl⟩
+    rw [PropFun.mem_semVars] at hv1 ⊢
+    rcases hv1 with ⟨τ,hpos,hneg⟩
+    rw [PropFun.satisfies_mk] at hpos hneg
+    have ⟨σ,h⟩ := τ.exists_preimage ⟨f,hf⟩
+    cases h; simp at hpos hneg
+    use σ
+    dsimp
+    rw [PropFun.satisfies_mk, PropFun.satisfies_mk]
+    simp [satisfies_map, hpos]
+    rw [PropAssignment.map_set]
+    · exact hneg
+    · assumption
+
+end map /- section -/
+
+end PropForm
+
+namespace PropFun
+
+def map (f : ν₁ → ν₂) (φ : PropFun ν₁) : PropFun ν₂ :=
+  φ.lift (⟦ PropForm.map f · ⟧) (by
+    intro a b h
+    simp
+    ext τ
+    rw [PropFun.satisfies_mk, PropFun.satisfies_mk]
+    simp [PropForm.satisfies_map]
+    rw [← PropFun.satisfies_mk, ← PropFun.satisfies_mk, Quotient.eq.mpr h]
+  )
+
+section map
+
+@[simp]
+theorem satisfies_map {φ : PropFun ν₁} {f} {τ : PropAssignment ν₂}
+    : τ ⊨ φ.map f ↔ (τ.map f) ⊨ φ := by
+  let ⟨ϕ,hϕ⟩ := φ.toTrunc.out
+  cases hϕ
+  simp [map]
+  rw [satisfies_mk, satisfies_mk]
+  apply PropForm.satisfies_map
+
+theorem semVars_map [DecidableEq ν₁] [DecidableEq ν₂] [Fintype ν₁]
+    (f : ν₁ → ν₂) (φ : PropFun ν₁) (hf : f.Injective)
+    : (φ.map f).semVars = φ.semVars.map ⟨f,hf⟩ := by
+  let ⟨ϕ,hϕ⟩ := φ.toTrunc.out; cases hϕ
+  simp [map, *, PropForm.semVars_map]
+
+variable (f : ν₁ → ν₂) (φ φ₁ φ₂ : PropFun ν₁)
+
+@[simp] theorem map_var (v : ν₁) : map f (.var v) = .var (f v) := rfl
+@[simp] theorem map_tr  : map f ⊤ = ⊤ := rfl
+@[simp] theorem map_fls : map f ⊥ = ⊥ := rfl
+@[simp] theorem map_neg  : map f (φᶜ) = (map f φ)ᶜ := by ext; simp
+@[simp] theorem map_conj : map f (φ₁ ⊓ φ₂) = (map f φ₁ ⊓ map f φ₂) := by ext; simp
+@[simp] theorem map_disj : map f (φ₁ ⊔ φ₂) = (map f φ₁ ⊔ map f φ₂) := by ext; simp
+@[simp] theorem map_impl : map f (φ₁ ⇨ φ₂) = (map f φ₁ ⇨ map f φ₂) := by ext; simp
+@[simp] theorem map_biImpl : map f (biImpl φ₁ φ₂) = .biImpl (map f φ₁) (map f φ₂) := by ext; simp
+
+end map /- section -/
+
+end PropFun
+
+end LeanSAT.Model
